src/sequential/SeqLiftAux.v
@@ -46,13 +46,34 @@ Require Import SeqLiftStep.
 
 
 
-Lemma mapped_msgs_exists_aux f0 f1 vers srctm flag_src flag_tgt msgs_tgt prom_src prom_tgt loc flag_new
-      (PROM: sim_promises srctm flag_src flag_tgt f0 vers prom_src prom_tgt)
+Lemma mapped_msgs_exists_aux f0 f1 vers msgs_tgt prom_tgt loc flag_new
+      mem_src
+      (PROM: exists srctm flag_src flag_tgt prom_src, sim_promises srctm flag_src flag_tgt f0 vers prom_src prom_tgt)
       (MAPLE: Mapping.le (f0 loc) f1)
       (MSGS: forall from to msg (IN: List.In (from, to, msg) msgs_tgt), Memory.get loc to prom_tgt = Some (from, msg))
       (WF0: Mapping.wfs f0)
       (WF1: Mapping.wf f1)
       (VERSWF: versions_wf f0 vers)
+      (BOTNONE: Memory.bot_none prom_tgt)
+      (MSGSWF: wf_cell_msgs msgs_tgt)
+      (SIM: sim_closed_memory f0 mem_src)
+
+      ts_tgt ts_src
+      (SIMTIME: sim_timestamp_exact f1 f1.(Mapping.ver) ts_src ts_tgt)
+      (MAX: Time.le (Memory.max_ts loc mem_src) ts_src)
+      (RESERVE: forall from_tgt to_tgt msg_tgt from_src to_src
+                       (GET: Memory.get loc to_tgt prom_tgt = Some (from_tgt, msg_tgt))
+                       (TS: Time.lt from_tgt ts_tgt)
+                       (TO: sim_timestamp_exact (f0 loc) (f0 loc).(Mapping.ver) to_src to_tgt)
+                       (FROM: sim_timestamp_exact (f0 loc) (f0 loc).(Mapping.ver) from_src from_tgt),
+          (<<RESERVE: msg_tgt = Message.reserve>>) /\
+          (<<TS: Time.lt to_tgt ts_tgt>>) /\
+          (<<DISJOINT: forall from to msg (GET: Memory.get loc to mem_src = Some (from, msg)),
+              Interval.disjoint (from_src, to_src) (from, to)>>))
+      (SAME: forall to_tgt to_src
+                    (TS: Time.lt to_tgt ts_tgt)
+                    (MAP: sim_timestamp_exact (f0 loc) (f0 loc).(Mapping.ver) to_src to_tgt),
+          sim_timestamp_exact f1 f1.(Mapping.ver) to_src to_tgt)
   :
     exists msgs_src,
       (<<FORALL: List.Forall2
@@ -60,11 +81,20 @@ Lemma mapped_msgs_exists_aux f0 f1 vers srctm flag_src flag_tgt msgs_tgt prom_sr
                       (<<FROM: sim_timestamp_exact f1 f1.(Mapping.ver) from_src from_tgt>>) /\
                       (<<TO: sim_timestamp_exact f1 f1.(Mapping.ver) to_src to_tgt>>) /\
                       (<<MESSAGE: sim_message_max flag_new loc to_src f0 (vers loc to_tgt) msg_src msg_tgt>>))
-                   msgs_src msgs_tgt>>).
+                   msgs_src msgs_tgt>>) /\
+      (<<DISJOINT: List.Forall
+                     (fun '(from, to, msg) => (__guard__((<<MAX: Time.le (Memory.max_ts loc mem_src) from>>) \/ (<<RESERVE: msg = Message.reserve>>) /\ (<<DISJOINT: forall to2 from2 msg2 (GET: Memory.get loc to2 mem_src = Some (from2, msg2)), Interval.disjoint (from, to) (from2, to2)>>))) /\ (<<TS: Time.lt from to>>) /\ (<<MSGTO: Memory.message_to msg loc to>>) /\ (<<WF: Message.wf msg>>) /\ (<<CLOSED: semi_closed_message msg mem_src loc to>>)) msgs_src>>) /\
+      (<<MSGSWF: wf_cell_msgs msgs_src>>)
+.
 Proof.
-  revert MSGS. induction msgs_tgt; i.
-  { exists []. red. econs. }
-  destruct a as [[from_tgt to_tgt] msg_tgt].
+  pose proof mapping_latest_wf_loc as VERWF.
+  revert MSGS MSGSWF. induction msgs_tgt; i.
+  { exists []. splits.
+    { econs. }
+    { econs. }
+    { red. splits; econs. }
+  }
+  des. destruct a as [[from_tgt to_tgt] msg_tgt].
   hexploit MSGS.
   { left. eauto. }
   intros GETTGT. hexploit sim_promises_get; eauto. i. des.
@@ -74,118 +104,93 @@ Proof.
   { i. hexploit VERS; eauto. i. des. esplits; eauto.
     exploit VERSWF. rewrite VER. ss.
   }
-  i. des.
+  i. des. red in MSGSWF. des. inv DISJOINT. inv MSGSWF0.
   hexploit IHmsgs_tgt; eauto.
   { i. eapply MSGS. right. auto. }
-  i. des. exists ((ts_src1, ts_src0, msg_src)::msgs_src).
-  red. econs; eauto.
-Qed.
-
-Lemma mapped_msgs_wf_msgs f0 f1 msgs_src msgs_tgt loc vers flag_new
-      (WF1: Mapping.wf f1)
-      (MSGSWF: wf_cell_msgs msgs_tgt)
-      (FORALL: List.Forall2
-                 (fun '(from_src, to_src, msg_src) '(from_tgt, to_tgt, msg_tgt) =>
-                    (<<FROM: sim_timestamp_exact f1 f1.(Mapping.ver) from_src from_tgt>>) /\
-                    (<<TO: sim_timestamp_exact f1 f1.(Mapping.ver) to_src to_tgt>>) /\
-                    (<<MESSAGE: sim_message_max flag_new loc to_src f0 (vers loc to_tgt) msg_src msg_tgt>>))
-                 msgs_src msgs_tgt)
-      (BOTNONE: List.Forall (fun '(_, to, _) => to <> Time.bot) msgs_tgt)
-  :
-    wf_cell_msgs msgs_src.
-Proof.
-  pose proof mapping_latest_wf_loc as VERWF.
-  red in MSGSWF. des.
-  revert msgs_src DISJOINT MSGSWF0 FORALL BOTNONE. induction msgs_tgt; i.
-  { inv FORALL. repeat red. splits.
-    { econs. }
-    { econs. }
+  { red. splits; auto. }
+  i. destruct H1 as [MSGWF TIMEWF]. guardH TIMEWF.
+  des.
+  assert (FROMTO: Time.lt ts_src1 ts_src0).
+  { eapply sim_timestamp_exact_lt; eauto.
+    hexploit memory_get_ts_strong; eauto. i. des; clarify.
+    rewrite BOTNONE in GETTGT. ss.
   }
-  inv FORALL. inv MSGSWF0. inv DISJOINT. inv BOTNONE.
-  destruct x as [[from_src to_src] msg_src]. des; clarify.
-  hexploit IHmsgs_tgt; eauto. i. repeat red in H. repeat red. des. econs.
-  { econs; eauto.
-    eapply List.Forall_forall. intros [[from_src0 to_src0] msg_src0] IN.
-    eapply list_Forall2_in2 in IN; eauto. des.
-    destruct b as [[from_tgt0 to_tgt0] msg_tgt0]. des.
-    eapply List.Forall_forall in HD; eauto. ss.
-    eapply sim_timestamp_exact_le; eauto.
-  }
-  { econs; eauto. split.
+  exists ((ts_src1, ts_src0, msg_src)::msgs_src). splits.
+  { econs; eauto. }
+  { econs; eauto. splits.
+    { destruct (Time.le_lt_dec ts_tgt from_tgt).
+      { left. transitivity ts_src; auto. eapply sim_timestamp_exact_le; eauto. }
+      { right. hexploit RESERVE; eauto. i. des. subst.
+        hexploit (@SAME to_tgt to_src); eauto. i.
+        eapply sim_timestamp_exact_inject in SIM1; eauto. subst.
+        hexploit (@SAME from_tgt from_src); eauto. i.
+        eapply sim_timestamp_exact_inject in SIM0; eauto. subst.
+        splits.
+        { inv MAX0; ss. }
+        { i. eauto. }
+      }
+    }
+    { auto. }
+    { eapply sim_message_max_msg_to; eauto. }
     { eapply sim_message_max_msg_wf; eauto. }
-    { right. eapply sim_timestamp_exact_lt; eauto. }
+    { eapply sim_closed_memory_sim_message; eauto. }
+  }
+  { red in MSGSWF. des. red. splits.
+    { econs; eauto.
+      eapply List.Forall_forall. intros [[from_src0 to_src0] msg_src0] IN.
+      eapply list_Forall2_in2 in IN; eauto. des.
+      destruct b as [[from_tgt0 to_tgt0] msg_tgt0]. des.
+      eapply List.Forall_forall in HD; eauto. ss.
+      eapply sim_timestamp_exact_le; eauto.
+    }
+    { econs; eauto. splits; auto.
+      eapply sim_message_max_msg_wf; eauto.
+    }
   }
 Qed.
 
-Lemma mapped_msgs_disjoint f0 f1 msgs_src msgs_tgt loc vers flag_new mem_src
-      ts_tgt ts_src
-      (WF1: Mapping.wf f1)
-      (MSGSWF: wf_cell_msgs msgs_tgt)
-      (FORALL: List.Forall2
-                 (fun '(from_src, to_src, msg_src) '(from_tgt, to_tgt, msg_tgt) =>
-                    (<<FROM: sim_timestamp_exact f1 f1.(Mapping.ver) from_src from_tgt>>) /\
-                    (<<TO: sim_timestamp_exact f1 f1.(Mapping.ver) to_src to_tgt>>) /\
-                    (<<MESSAGE: sim_message_max flag_new loc to_src f0 (vers loc to_tgt) msg_src msg_tgt>>))
-                 msgs_src msgs_tgt)
-      (BOTNONE: List.Forall (fun '(_, to, _) => to <> Time.bot) msgs_tgt)
-
-
-      (TS
-
+Lemma messages_times_exists (msgs: list (Time.t * Time.t * Message.t)) (f0: Mapping.t) ts
+      (MAPWF: Mapping.wf f0)
   :
-    List.Forall
-      (fun '(from, to, msg) => (__guard__((<<MAX: Time.le (Memory.max_ts loc mem_src) from>>) \/ (<<RESERVE: msg = Message.reserve>>) /\ (<<DISJOINT: forall to2 from2 msg2 (GET: Memory.get loc to2 mem_src = Some (from2, msg2)), Interval.disjoint (from, to) (from2, to2)>>))) /\ (<<TS: Time.lt from to>>) /\ (<<MSGTO: Memory.message_to msg loc to>>) /\ (<<WF: Message.wf msg>>) /\ (<<CLOSED: semi_closed_message msg mem_src loc to>>)) msgs_src.
-Proof.
-
-
-shifted_mapping_exists
-
-
-Lemma mapped_msgs_wf_msgs f0 f1 msgs_src msgs_tgt loc vers flag_new
-      mem_src
-      (WF1: Mapping.wf f1)
-      (MSGSWF: wf_cell_msgs msgs_tgt)
-      (FORALL: List.Forall2
-                 (fun '(from_src, to_src, msg_src) '(from_tgt, to_tgt, msg_tgt) =>
-                    (<<FROM: sim_timestamp_exact f1 f1.(Mapping.ver) from_src from_tgt>>) /\
-                    (<<TO: sim_timestamp_exact f1 f1.(Mapping.ver) to_src to_tgt>>) /\
-                    (<<MESSAGE: sim_message_max flag_new loc to_src f0 (vers loc to_tgt) msg_src msg_tgt>>))
-                 msgs_src msgs_tgt)
-      (BOTNONE: List.Forall (fun '(_, to, _) => to <> Time.bot) msgs_tgt)
-  :
-    (<<MSGSWF: wf_cell_msgs msgs_src>>) /\
-    (<<MSGS: List.Forall
-               (fun '(from, to, msg) => (__guard__((<<MAX: Time.le (Memory.max_ts loc mem_src) from>>) \/ (<<RESERVE: msg = Message.reserve>>) /\ (<<DISJOINT: forall to2 from2 msg2 (GET: Memory.get loc to2 mem_src = Some (from2, msg2)), Interval.disjoint (from, to) (from2, to2)>>))) /\ (<<TS: Time.lt from to>>) /\ (<<MSGTO: Memory.message_to msg loc to>>) /\ (<<WF: Message.wf msg>>) /\ (<<CLOSED: semi_closed_message msg mem_src loc to>>)) msgs_src>>)
+    exists (f1: Mapping.t),
+      (<<MAPWF: Mapping.wf f1>>) /\
+      (<<MAPLE: Mapping.le_strong f0 f1>>) /\
+      (<<CLOSEDIF: forall to (CLOSED: Mapping.closed f1 f1.(Mapping.ver) to),
+          (<<CLOSED: Mapping.closed f0 f0.(Mapping.ver) to>>) \/
+          (exists from val released, (<<IN: List.In (from, to, Message.concrete val released) msgs>>)) \/
+          (<<TS: to = ts>>)>>) /\
+      (<<CLOSED: List.Forall (fun '(from_src, to_src, msg_src) =>
+                                forall val released (MSG: msg_src = Message.concrete val released),
+                                  Mapping.closed f1 f1.(Mapping.ver) to_src) msgs>>) /\
+      (<<CLOSEDTS: Mapping.closed f1 f1.(Mapping.ver) ts>>)
 .
 Proof.
-  pose proof mapping_latest_wf_loc as VERWF.
-  red in MSGSWF. des.
-  revert msgs_src DISJOINT MSGSWF0 FORALL BOTNONE. induction msgs_tgt; i.
-  { inv FORALL. repeat red. splits.
-    { econs. }
-    { econs. }
+  hexploit (@mapping_update_times f0 (fun to => to = ts \/ exists from val released, List.In (from, to, Message.concrete val released) msgs)).
+  { eauto. }
+  { induction msgs.
+    { exists [ts]. i. des; ss; auto. }
+    { des. destruct a as [[from to] msg]. destruct msg.
+      { exists (to::l). i. ss. des; clarify.
+        { right. eapply IHmsgs. left. auto. }
+        { auto. }
+        { right. eapply IHmsgs. right. eauto. }
+      }
+      { exists l. i. eapply IHmsgs. ss. des; clarify; eauto. }
+      { exists l. i. eapply IHmsgs. ss. des; clarify; eauto. }
+    }
   }
-  inv FORALL. inv MSGSWF0. inv DISJOINT. inv BOTNONE.
-  destruct x as [[from_src to_src] msg_src]. des; clarify.
-  hexploit IHmsgs_tgt; eauto. i. repeat red in H. repeat red. des. econs.
-  { econs; eauto.
-    eapply List.Forall_forall. intros [[from_src0 to_src0] msg_src0] IN.
-    eapply list_Forall2_in2 in IN; eauto. des.
-    destruct b as [[from_tgt0 to_tgt0] msg_tgt0]. des.
-    eapply List.Forall_forall in HD; eauto. ss.
-    eapply sim_timestamp_exact_le; eauto.
+  i. des. exists f1. splits; eauto.
+  { i. eapply TIMES in CLOSED. des; auto.
+    right. esplits; eauto.
   }
-  { econs; eauto. split.
-    { eapply sim_message_max_msg_wf; eauto. }
-    { right. eapply sim_timestamp_exact_lt; eauto. }
+  { eapply List.Forall_forall. intros [[from to] msg] IN. i. subst.
+    eapply TIMES. right. esplits; eauto.
   }
+  { eapply TIMES. right. left. auto. }
 Qed.
-
-
 
 Lemma mapped_msgs_complete f0 f1 msgs_src msgs_tgt loc vers flag_new
       (WF1: Mapping.wf f1)
-      (MSGSWF: wf_cell_msgs msgs_tgt)
       (FORALL: List.Forall2
                  (fun '(from_src, to_src, msg_src) '(from_tgt, to_tgt, msg_tgt) =>
                     (<<FROM: sim_timestamp_exact f1 f1.(Mapping.ver) from_src from_tgt>>) /\
@@ -215,7 +220,6 @@ Qed.
 
 Lemma mapped_msgs_sound f0 f1 msgs_src msgs_tgt loc vers flag_new
       (WF1: Mapping.wf f1)
-      (MSGSWF: wf_cell_msgs msgs_tgt)
       (FORALL: List.Forall2
                  (fun '(from_src, to_src, msg_src) '(from_tgt, to_tgt, msg_tgt) =>
                     (<<FROM: sim_timestamp_exact f1 f1.(Mapping.ver) from_src from_tgt>>) /\
@@ -236,7 +240,6 @@ Qed.
 
 Lemma mapped_msgs_complete_promise f0 f1 msgs_src msgs_tgt loc vers flag_new
       (WF1: Mapping.wf f1)
-      (MSGSWF: wf_cell_msgs msgs_tgt)
       (FORALL: List.Forall2
                  (fun '(from_src, to_src, msg_src) '(from_tgt, to_tgt, msg_tgt) =>
                     (<<FROM: sim_timestamp_exact f1 f1.(Mapping.ver) from_src from_tgt>>) /\
@@ -263,7 +266,6 @@ Qed.
 
 Lemma mapped_msgs_sound_promise f0 f1 msgs_src msgs_tgt loc vers flag_new
       (WF1: Mapping.wf f1)
-      (MSGSWF: wf_cell_msgs msgs_tgt)
       (FORALL: List.Forall2
                  (fun '(from_src, to_src, msg_src) '(from_tgt, to_tgt, msg_tgt) =>
                     (<<FROM: sim_timestamp_exact f1 f1.(Mapping.ver) from_src from_tgt>>) /\
@@ -285,40 +287,6 @@ Proof.
   destruct b as [[from_tgt to_tgt] msg_tgt]. des. esplits; eauto.
 Qed.
 
-Lemma mapped_msgs_disjoint f0 f1 msgs_src msgs_tgt loc vers flag_new mem_src
-      (WF1: Mapping.wf f1)
-      (MSGSWF: wf_cell_msgs msgs_tgt)
-      (FORALL: List.Forall2
-                 (fun '(from_src, to_src, msg_src) '(from_tgt, to_tgt, msg_tgt) =>
-                    (<<FROM: sim_timestamp_exact f1 f1.(Mapping.ver) from_src from_tgt>>) /\
-                    (<<TO: sim_timestamp_exact f1 f1.(Mapping.ver) to_src to_tgt>>) /\
-                    (<<MESSAGE: sim_message_max flag_new loc to_src f0 (vers loc to_tgt) msg_src msg_tgt>>))
-                 msgs_src msgs_tgt)
-  :
-    List.Forall
-      (fun '(from, to, msg) => (__guard__((<<MAX: Time.le (Memory.max_ts loc mem_src) from>>) \/ (<<RESERVE: msg = Message.reserve>>) /\ (<<DISJOINT: forall to2 from2 msg2 (GET: Memory.get loc to2 mem_src = Some (from2, msg2)), Interval.disjoint (from, to) (from2, to2)>>))) /\ (<<TS: Time.lt from to>>) /\ (<<MSGTO: Memory.message_to msg loc to>>) /\ (<<WF: Message.wf msg>>) /\ (<<CLOSED: semi_closed_message msg mem_src loc to>>)) msgs_src.
-Proof.
-  i. eapply List.Forall_forall. i.
-  eapply list_Forall2_in2 in H; eauto. des.
-  destruct b as [[from_tgt to_tgt] msg_tgt].
-  destruct x as [[from_src to_src] msg_src]. des. esplits; eauto.
-
-
-
-    forall to_src from_src msg_src
-           (IN: List.In (from_src, to_src, msg_src) msgs_src),
-    exists to_tgt from_tgt msg_tgt,
-      (<<TO: sim_timestamp_exact f1 f1.(Mapping.ver) to_src to_tgt>>) /\
-      (<<FROM: sim_timestamp_exact f1 f1.(Mapping.ver) from_src from_tgt>>) /\
-      (<<GET: List.In (from_tgt, to_tgt, msg_tgt) msgs_tgt>>).
-Proof.
-  i. eapply list_Forall2_in2 in IN; eauto. des.
-  destruct b as [[from_tgt to_tgt] msg_tgt]. des. esplits; eauto.
-Qed.
-
-List.Forall
-                    (fun '(from, to, msg) => (__guard__((<<MAX: Time.le (Memory.max_ts loc mem0) from>>) \/ (<<RESERVE: msg = Message.reserve>>) /\ (<<DISJOINT: forall to2 from2 msg2 (GET: Memory.get loc to2 mem0 = Some (from2, msg2)), Interval.disjoint (from, to) (from2, to2)>>))) /\ (<<TS: Time.lt from to>>) /\ (<<MSGTO: Memory.message_to msg loc to>>) /\ (<<WF: Message.wf msg>>) /\ (<<CLOSED: semi_closed_message msg mem0 loc to>>)) msgs
-
 Lemma sim_thread_deflag_match_aux2
       f0 vers flag_src flag_tgt vs_src vs_tgt
       mem_src0 mem_tgt lc_src0 lc_tgt sc_src sc_tgt
@@ -334,6 +302,7 @@ Lemma sim_thread_deflag_match_aux2
       (SCSRC: Memory.closed_timemap sc_src mem_src0)
       (SCTGT: Memory.closed_timemap sc_tgt mem_tgt)
       (WF: Mapping.wfs f0)
+      (VERSWF: versions_wf f0 vers)
       (FLAG: flag_src loc = true)
       (VAL: option_rel Const.le (vs_tgt loc) (vs_src loc))
       lang st
@@ -365,41 +334,214 @@ Proof.
   assert (TS: srctm loc = View.rlx (TView.cur tvw) loc).
   { inv LOCAL. auto. }
   hexploit sim_memory_top; eauto. intros TOP.
-  hexploit (@shifted_mapping_exists (f0 loc) (srctm loc)); eauto. i. des.
+  hexploit (@shifted_mapping_exists (f0 loc) (View.pln (TView.cur tvw0) loc) (srctm loc)); eauto. i. des.
+  hexploit (@wf_cell_msgs_exists (prom0 loc)). intros [msgs_tgt ?]. des.
+  hexploit mapped_msgs_exists_aux.
+  { inv LOCAL. eauto. }
+  { eauto. }
+  { i. eapply COMPLETE. eauto. }
+  { eauto. }
+  { eauto. }
+  { eauto. }
+  { eapply LOCALTGT. }
+  { eauto. }
+  { eauto. }
+  { eapply TS0. }
+  { inv LOCAL. rewrite MAXTIMES; auto. refl. }
+  { admit. }
+  { eauto. }
+  i. des.
+  inv MAX0. inv MAX2. ss.
+  hexploit sim_memory_sound; eauto. i. des.
+  { exfalso. eapply TOP in TO. eapply Time.lt_strorder.
+    eapply TimeFacts.lt_le_lt.
+    { eapply TO. }
+    { inv LOCAL. rewrite SRCTM. rewrite FLAGSRC; auto. }
+  }
+  hexploit NONE1; eauto. i. subst.
+  hexploit (messages_times_exists msgs_src f1); auto. i. des.
+  eapply list_Forall2_impl in FORALL; cycle 1.
+  { i. instantiate (1:= fun '(from_src, to_src, msg_src) '(from_tgt, to_tgt, msg_tgt) =>
+                          (<<FROM: sim_timestamp_exact f2 f2.(Mapping.ver) from_src from_tgt>>) /\
+                          (<<TO: sim_timestamp_exact f2 f2.(Mapping.ver) to_src to_tgt>>) /\
+                          (<<MESSAGE: sim_message_max false loc to_src f0 (vers loc to_tgt) msg_src msg_tgt>>)).
+    destruct a as [[from_src to_src] msg_src]. destruct b as [[from_tgt to_tgt] msg_tgt].
+    des. splits; eauto.
+    { eapply sim_timestamp_exact_mon_strong; [..|eauto]; eauto.  }
+    { eapply sim_timestamp_exact_mon_strong; [..|eauto]; eauto.  }
+  }
+  pose proof (mapped_msgs_complete _ _ _ _ _ _ _ MAPWF FORALL CLOSED0) as COMPLETEMEM.
+  pose proof (mapped_msgs_sound _ _ _ _ _ _ _ MAPWF FORALL) as SOUNDMEM.
+  pose proof (mapped_msgs_complete_promise _ _ _ _ _ _ _ MAPWF FORALL) as COMPLETEPROM.
+  pose proof (mapped_msgs_sound_promise _ _ _ _ _ _ _ MAPWF FORALL) as SOUNDPROM.
+  set (f' := fun loc0 => if Loc.eq_dec loc0 loc then f2 else f0 loc0).
+  assert (MAPSLE: Mapping.les f0 f').
+  { unfold f'. ii. condtac; subst.
+    { etrans; eauto. eapply Mapping.le_strong_le; eauto. }
+    { refl. }
+  }
+  assert (MAPSWF: Mapping.wfs f').
+  { unfold f'. ii. condtac; subst; eauto. }
+  hexploit add_promises_latest.
+  { eapply MSGSWF. }
+  { eapply LOCALSRC. }
+  { eapply MEMSRC. }
+  { eauto. }
+  i. des. inv LOCAL.
+  hexploit added_memory_sim_memory; eauto.
+  { rewrite TS. rewrite FLAGSRC; eauto. }
+  {  hexploit sim_memory_get; eauto; ss. i. des.
+     inv MSG; econs; eauto; econs.
+  }
+  { ss. }
+  { i. eapply MAX0 in GETTGT; eauto.
+    eapply COMPLETE in GETTGT. eapply COMPLETEMEM; eauto.
+  }
+  { i. eapply SOUNDMEM in IN. des. esplits; eauto.
+    eapply LOCALTGT. eapply COMPLETE; eauto.
+  }
+  { etrans; eauto. eapply Mapping.le_strong_le; eauto. }
+  { i. eapply sim_timestamp_exact_mon_strong; [|eauto|..]; eauto. }
+  { eapply sim_timestamp_exact_mon_strong; [|eauto|..]; eauto. }
+  { i. eapply CLOSEDIF in CLOSED1. des.
+    { left. eapply CLOSED. auto. }
+    { right. left. eauto. }
+    { subst. right. right. esplits; eauto. }
+  }
+  i. destruct H as [MEM1 ?]. des.
+  esplits.
+  { eapply STEPS. }
+  { econs.
+    { instantiate (1:=f'). eapply sim_timemap_mon_latest; eauto. }
+    { eapply added_memory_sim_memory; eauto.
+      { rewrite TS. rewrite FLAGSRC; eauto. }
+      {  hexploit sim_memory_get; eauto; ss. i. des.
+         inv MSG; econs; eauto; econs.
+      }
+      { ss. }
+      { i. eapply MAX0 in GETTGT; eauto.
+        eapply COMPLETE in GETTGT. eapply COMPLETEMEM; eauto.
+      }
+      { i. eapply SOUNDMEM in IN. des. esplits; eauto.
+        eapply LOCALTGT. eapply COMPLETE; eauto.
+      }
+      { etrans; eauto. eapply Mapping.le_strong_le; eauto. }
+      { i. eapply sim_timestamp_exact_mon_strong; [|eauto|..]; eauto. }
+      { eapply sim_timestamp_exact_mon_strong; [|eauto|..]; eauto. }
+      { i. eapply CLOSEDIF in CLOSED1. des.
+        { left. eapply CLOSED. auto. }
+        { right. left. eauto. }
+        { subst. right. right. esplits; eauto. }
+      }
+    }
+    { econs.
+      { admit. }
+      { eapply added_memory_sim_promise_match; eauto.
+        { i. eapply COMPLETE in GETTGT. eapply COMPLETEPROM in GETTGT; eauto. }
+        { i. eapply SOUNDPROM in IN; eauto. des.
+          esplits; eauto. eapply COMPLETE; eauto.
+        }
+        { etrans; eauto. eapply Mapping.le_strong_le; eauto. }
+      }
+      { eauto. }
+      { i. des_ifs. eauto. }
+      { eauto. }
+    }
+    { admit. }
+    { eauto. }
+    { eauto. }
+    { red in FIN. des.
+      hexploit (list_filter_exists (fun loc0 => loc0 <> loc) dom). i. des.
+      exists l'. splits. i. etrans; [|eapply COMPLETE0]. condtac; subst.
+      { split; i; des; ss. }
+      { split; i.
+        { split; auto. eapply DOM; auto. }
+        { des. eapply DOM; eauto. }
+      }
+    }
+    { eauto. }
+    { eauto. }
+    { i. des_ifs. admit. }
+  }
+  { eauto. }
+  { eauto. }
+  { i. unfold f'. des_ifs. }
+  { eauto. }
+  { econs. unfold f'. i. des_ifs.
+    { destruct (Time.le_lt_dec (srctm loc) to_tgt).
+      { admit. }
+      { rewrite SRCTM in l. rewrite FLAGSRC in l; eauto.
+        eapply SAME in TO0; eauto.
 
-  hexploit
+
+        eapply SAME in FROM1.
+
+ admit.
+
+}
+    { eapply sim_timestamp_exact_inject in FROM0; eauto.
+      eapply sim_timestamp_exact_inject in TO0; eauto. subst. splits; auto.
+      inv MEM0. inv COVERED. rewrite OTHER in GET1; eauto. econs; eauto.
+    }
+  }
 
 
-    (MSGCOMPLETE: forall to_tgt from_tgt msg_tgt
-                         (GETTGT: Memory.get loc to_tgt prom_tgt = Some (from_tgt, msg_tgt)),
-        exists to_src from_src msg_src,
-          (<<TO: sim_timestamp_exact f1 f1.(Mapping.ver) to_src to_tgt>>) /\
-          (<<MSG: sim_message_max false loc to_src f0 (vers loc to_tgt) msg_src msg_tgt>>) /\
-          (<<CLOSED: Mapping.closed f1 f1.(Mapping.ver) to_src>>) /\
-          (<<IN: List.In (from_src, to_src, msg_src) msgs>>))
-    (MSGSOUND: forall to_src from_src msg_src
-                      (IN: List.In (from_src, to_src, msg_src) msgs),
-        exists to_tgt from_tgt msg_tgt,
-          (<<TO: sim_timestamp_exact f1 f1.(Mapping.ver) to_src to_tgt>>) /\
-          (<<FROM: sim_timestamp_exact f1 f1.(Mapping.ver) from_src from_tgt>>) /\
-          (<<GET: Memory.get loc to_tgt prom_tgt = Some (from_tgt, msg_tgt)>>))
+ss.
 
-    (CLOSEDIF: forall ts (CLOSED: Mapping.closed f1 f1.(Mapping.ver) ts),
-        (<<CLOSED: Mapping.closed (f0 loc) (f0 loc).(Mapping.ver) ts>>) \/
-        (exists from val released, (<<IN: List.In (from, ts, Message.concrete val released) msgs>>)))
+inv MSGS.
 
-         (FORALL: List.Forall
-                    (fun '(from, to, msg) => (__guard__((<<MAX: Time.le (Memory.max_ts loc mem0) from>>) \/ (<<RESERVE: msg = Message.reserve>>) /\ (<<DISJOINT: forall to2 from2 msg2 (GET: Memory.get loc to2 mem0 = Some (from2, msg2)), Interval.disjoint (from, to) (from2, to2)>>))) /\ (<<TS: Time.lt from to>>) /\ (<<MSGTO: Memory.message_to msg loc to>>) /\ (<<WF: Message.wf msg>>) /\ (<<CLOSED: semi_closed_message msg mem0 loc to>>)) msgs),
+ eauto. }
 
+ eauto.
+
+eauto.
 
 
 
-  wf_cell_msgs
-
-add_promises_latest
+eapply COMPLETE in GETTGT. eapply COMPLETEPROM in GETTGT; eauto. }
 
 
-Admitted.
+
+        3:{
+eapply MAX0 in GETTGT; eauto.
+        eapply COMPLETE in GETTGT. eapply COMPLETEMEM; eauto.
+      }
+
+in GETTGT; eauto.
+
+
+econs. assert (released = None).
+        { admit. }
+        { admit. }
+        sim_memory
+
+        subst. econs.
+released 4 with None.
+
+econs. eauto.
+
+eauto.
+
+sim_memory sim_closed_memory eauto.
+
+ eauto.
+
+
+  hexploit mapped_msgs_complete.
+  { eapply MAPWF. }
+  { eapply FORALL. }
+  { eapply CLOSED0. }
+eauto. }
+  { eauto. }
+  {
+
+eapply list_Forall2_impl; eaut.
+    {
+
+
+/ List.Forall_impl.
+
+  hexploit messages_times_exists.
 
 
 Lemma sim_thread_deflag_match_aux2
